Examples.v
@@ -1,0 +1,129 @@
+Add LoadPath "lib" as Lib.
+Require Import Lib.Neuromorphic Lib.Leak Lib.NoLeak.
+Require Import Arith List String Logic ZArith.
+Import ListNotations.
+Open Scope Z_scope.
+Open Scope string_scope.
+
+Module Examples.
+
+Definition in1 := Neuromorphic.neuron "A" 1.
+Definition in2 := Neuromorphic.neuron "B" 1.
+Definition inputs (a b : bool) := Neuromorphic.encode (Neuromorphic.encode [] in1 a) in2 b.
+
+(**** Examples with Leak ****)
+Module OrLeak.
+Definition out := Neuromorphic.neuron "A|B" 1.
+Definition synapses := [(in1, out, 1);(in2, out, 1)].
+Definition initial_state (a b : bool) := Neuromorphic.pair (inputs a b) synapses.
+
+Example computes_in_one_step: forall a b, Leak.eval 1 (initial_state a b) out = orb a b.
+Proof. destruct a, b; auto. Qed.
+Example clears_in_two_steps: forall a b, Leak.eval 2 (initial_state a b) out = false.
+Proof. destruct a, b; auto. Qed.
+Example potential_leaks:
+    forall (a b : bool) (n : Neuromorphic.Neuron),
+    Neuromorphic.plookup (Neuromorphic.get_potentials (Leak.step_n 2 (initial_state a b))) n = 0.
+Proof. destruct a, b; auto. Qed.
+End OrLeak.
+
+Module AndLeak.
+Definition out := Neuromorphic.neuron "A&B" 2.
+Definition synapses := [(in1, out, 1);(in2, out, 1)].
+Definition initial_state (a b : bool) := Neuromorphic.pair (inputs a b) synapses.
+
+Example computes_in_one_step: forall a b, Leak.eval 1 (initial_state a b) out = andb a b.
+Proof. destruct a, b; auto. Qed.
+Example clears_in_two_steps: forall a b, Leak.eval 2 (initial_state a b) out = false.
+Proof. destruct a, b; auto. Qed.
+Example potential_leaks:
+    forall (a b : bool) (n : Neuromorphic.Neuron),
+    Neuromorphic.plookup (Neuromorphic.get_potentials (Leak.step_n 2 (initial_state a b))) n = 0.
+Proof. destruct a, b; auto. Qed.
+
+(*
+We want to show that computing (a, b) = (1, 0) and (a, b) = (0, 1) one after the other results in
+correct output due to potentials leaking. i.e. node "A&B" leaks the half potential of 1 before it
+is fired again
+*)
+Example and_leak_correct:
+    Leak.eval 1 (initial_state true false) out = false /\
+    Leak.eval 1 (Neuromorphic.update_state (Leak.step (initial_state true false)) in2 1) out = false.
+Proof. auto. Qed.
+Example and_leak_correct_reverse:
+    Leak.eval 1 (initial_state false true) out = false /\
+    Leak.eval 1 (Neuromorphic.update_state (Leak.step (initial_state false true)) in1 1) out = false.
+Proof. auto. Qed.
+End AndLeak.
+
+Module XorLeak.
+Definition h1 := Neuromorphic.neuron "A&~B" 1.
+Definition h2 := Neuromorphic.neuron "B&~A" 1.
+Definition out := Neuromorphic.neuron "A^B" 1.
+Definition synapses := [(in1, h1, 1);(in1, h2, (-1));(in2, h1, (-1));(in2, h2, 1);(h1, out, 1);(h2, out, 1)].
+Definition initial_state (a b : bool) := Neuromorphic.pair (inputs a b) synapses.
+
+Example computes_in_two_steps: forall a b, Leak.eval 2 (initial_state a b) out = xorb a b.
+Proof. destruct a, b; auto. Qed.
+Example clears_in_three_steps: forall a b, Leak.eval 3 (initial_state a b) out = false.
+Proof. destruct a, b; auto. Qed.
+Example potential_leaks:
+    forall (a b : bool) (n : Neuromorphic.Neuron),
+    Neuromorphic.plookup (Neuromorphic.get_potentials (Leak.step_n 3 (initial_state a b))) n = 0.
+Proof. destruct a, b; auto. Qed.
+End XorLeak.
+
+(**** Examples without Leak ****)
+Module OrNoLeak.
+Definition out := Neuromorphic.neuron "A|B" 1.
+Definition synapses := [(in1, out, 1);(in2, out, 1)].
+Definition initial_state (a b : bool) := Neuromorphic.pair (inputs a b) synapses.
+
+Example computes_in_one_step: forall a b, NoLeak.eval 1 (initial_state a b) out = orb a b.
+Proof. destruct a, b; auto. Qed.
+Example clears_in_two_steps: forall a b, NoLeak.eval 2 (initial_state a b) out = false.
+Proof. destruct a, b; auto. Qed.
+Example potential_resets:
+    forall (a b : bool),
+    Neuromorphic.plookup (Neuromorphic.get_potentials (NoLeak.step_n 2 (initial_state a b))) in1 = 0 /\
+    Neuromorphic.plookup (Neuromorphic.get_potentials (NoLeak.step_n 2 (initial_state a b))) in2 = 0 /\
+    Neuromorphic.plookup (Neuromorphic.get_potentials (NoLeak.step_n 2 (initial_state a b))) out = 0.
+Proof. destruct a, b; auto. Qed.
+End OrNoLeak.
+
+Module AndNoLeak.
+Definition t1 := Neuromorphic.neuron "Ta" 1.
+Definition t2 := Neuromorphic.neuron "Tb" 1.
+Definition h1 := Neuromorphic.neuron "Ha" 1.
+Definition h2 := Neuromorphic.neuron "Hb" 1.
+Definition out := Neuromorphic.neuron "A&B" 2.
+Definition synapses :=  [(in1, t1, 1);(in2, t2, 1);(t1, h1, 1);(t2, h2, 1);
+                         (in1, out, 1);(in2, out, 1);(h1, out, (-1));(h2, out, (-1));
+                         (out, h1, (-1));(out, h2, (-1))].
+Definition initial_state (a b : bool) := Neuromorphic.pair (inputs a b) synapses.
+
+Example computes_in_one_step: forall a b, NoLeak.eval 1 (initial_state a b) out = andb a b.
+Proof. destruct a, b; auto. Qed.
+Example clears_in_three_steps:
+    forall a b,
+        Neuromorphic.plookup (Neuromorphic.get_potentials (NoLeak.step_n 3 (initial_state a b))) out = 0.
+Proof. destruct a, b; auto. Qed.
+End AndNoLeak.
+
+Module XorNoLeak.
+Definition h1 := Neuromorphic.neuron "A&~B" 1.
+Definition h2 := Neuromorphic.neuron "B&~A" 1.
+Definition out := Neuromorphic.neuron "A^B" 1.
+Definition synapses := [(in1, h1, 1);(in2, h2, 1);(h1, out, 1);(h2, out, 1);(out, out, 0);
+                        (h1, h2, 1);(h2, h1, 1);(in1, h2, (-1));(in2, h1, (-1))].
+Definition initial_state (a b : bool) := Neuromorphic.pair (inputs a b) synapses.
+
+Example computes_in_two_steps: forall a b, NoLeak.eval 2 (initial_state a b) out = xorb a b.
+Proof. destruct a, b; auto. Qed.
+Example clears_in_three_steps:
+forall a b,
+    Neuromorphic.plookup (Neuromorphic.get_potentials (NoLeak.step_n 3 (initial_state a b))) out = 0.
+Proof. destruct a, b; auto. Qed.
+End XorNoLeak.
+
+End Examples.
