lib/Leak.v
@@ -1,0 +1,37 @@
+Add LoadPath "lib" as Lib.
+Require Import Lib.Neuromorphic.
+Require Import Arith List String Logic ZArith.
+Import ListNotations.
+Open Scope Z_scope.
+Open Scope string_scope.
+
+Module Leak.
+(*
+We assume all neruons leak their potential after one timestep.
+Given an input state,
+step one timestep and return resulting state
+    1) Identify all neurons above threshold
+    2) Fire neurons we found
+*)
+Fixpoint step' (p : Neuromorphic.potentials) (g : Neuromorphic.graph) : Neuromorphic.potentials :=
+    match g with
+    | [] => [] (* no synapses left to fire *)
+    | (n1, n2, w) :: g' =>
+        if Neuromorphic.decode p n1 then
+        Neuromorphic.add_potential (step' p g') n2 w (* n1 should fire this synapse, add weight to n2 *)
+        else step' p g' (* this synapse is not fired *)
+    end.
+Definition step (st : Neuromorphic.state) : Neuromorphic.state :=
+    Neuromorphic.pair (step' (Neuromorphic.get_potentials st) (Neuromorphic.get_graph st)) (Neuromorphic.get_graph st).
+
+Fixpoint step_n (n: nat) (st: Neuromorphic.state) : Neuromorphic.state :=
+    match n with
+    | O => st
+    | S n' => step_n n' (step st)
+    end.
+
+(* run for n steps and check if neuron out has potential >= threshold *)
+Definition eval (steps : nat) (st : Neuromorphic.state) (out : Neuromorphic.Neuron) : bool :=
+    Neuromorphic.decode (Neuromorphic.get_potentials (step_n steps st)) out.
+
+End Leak.
