lib/NoLeak.v
@@ -1,0 +1,60 @@
+Add LoadPath "lib" as Lib.
+Require Import Lib.Neuromorphic.
+Require Import Arith List String Logic ZArith.
+Import ListNotations.
+Open Scope Z_scope.
+Open Scope string_scope.
+
+Module NoLeak.
+(*
+Given an input state,
+step one timestep and return resulting state
+    1) Identify all neurons above threshold
+    2) Fire neurons we found
+*)
+Fixpoint step' (p : Neuromorphic.potentials) (g : Neuromorphic.graph) : Neuromorphic.potentials :=
+    match g with
+    | [] => [] (* no synapses left to fire *)
+    | (n1, n2, w) :: g' =>
+        if Neuromorphic.decode p n1 then
+        Neuromorphic.add_potential (step' p g') n2 w (* n1 should fire this synapse, add weight to n2 *)
+
+        (*
+        this synapse is not fired, it should not lose it's potential
+        when making recursive call, set potential for n1 to 0 so that we don't double count
+        *)
+        else
+        Neuromorphic.add_potential (step' (Neuromorphic.reset_potential p n1) g') n1 (Neuromorphic.plookup p n1)
+    end.
+Definition step (st : Neuromorphic.state) : Neuromorphic.state :=
+    Neuromorphic.pair (step' (Neuromorphic.get_potentials st) (Neuromorphic.get_graph st)) (Neuromorphic.get_graph st).
+
+Fixpoint step_n (n: nat) (st: Neuromorphic.state) : Neuromorphic.state :=
+    match n with
+    | O => st
+    | S n' => step_n n' (step st)
+    end.
+
+(* run for n steps and check if neuron out has potential >= threshold *)
+Definition eval (steps : nat) (st : Neuromorphic.state) (out : Neuromorphic.Neuron) : bool :=
+    Neuromorphic.decode (Neuromorphic.get_potentials (step_n steps st)) out.
+    
+Module TestNoLeak.
+Definition a := Neuromorphic.neuron "A" 1.
+Definition b := Neuromorphic.neuron "B" 2.
+Definition inputs := Neuromorphic.encode [] a true.
+Definition synapses := Neuromorphic.set_synapse (Neuromorphic.set_synapse [] b b 0) a b 1.
+Definition initial_state := Neuromorphic.pair inputs synapses.
+Example values_after_one_step:
+    Neuromorphic.plookup (Neuromorphic.get_potentials (step initial_state)) a = 0 /\
+    Neuromorphic.plookup (Neuromorphic.get_potentials (step initial_state)) b = 1.
+Proof. auto. Qed.
+Example b_does_not_fire: eval 1 initial_state b = false.
+Proof. auto. Qed.
+Example values_after_two_steps:
+    Neuromorphic.plookup (Neuromorphic.get_potentials (step_n 2 initial_state)) a = 0 /\
+    Neuromorphic.plookup (Neuromorphic.get_potentials (step_n 2 initial_state)) b = 1.
+Proof. auto. Qed.
+End TestNoLeak.
+
+End NoLeak.
