Makefile
@@ -1,0 +1,20 @@
+LIB_NAME=Lib
+LIB_DIR=lib
+
+# TODO(nikita): we want Neuromorphic.v to compile first so we
+# hardcode the order for now
+# LIB_FILES=${wildcard ${LIB_DIR}/*.v}
+LIB_FILES=lib/Neuromorphic.v lib/Leak.v lib/NoLeak.v
+LIB_BASE=${basename ${LIB_FILES}}
+LIB_VO_FILES=${addsuffix .vo,${LIB_BASE}}
+
+CC=coqc
+CFLAGS=-R ${LIB_DIR} ${LIB_NAME}
+
+lib: ${LIB_VO_FILES} Makefile ;
+
+${LIB_VO_FILES} : lib/%.vo : Makefile lib/%.v
+	${CC} ${CFLAGS} lib/$*.v
+
+clean:
+	rm -f lib/.*.aux lib/*.vo lib/*.vok lib/*.vos lib/*.glob
